Add more perf experiments, rework Harness

performance-experiments/Harness.v
@@ -108,6 +108,63 @@ End NatFstOrder.
 Module NatFstSort := Sort NatFstOrder.
 Notation sort_by_fst := NatFstSort.sort.
 
+Module ZProdOrder <: TotalLeBool.
+  Local Open Scope Z_scope.
+  Definition t := (Z * Z)%type.
+  Definition t_to_Z (v : t) : Z := (fst v * snd v)%Z.
+  Definition ltb (x y : t) : bool
+    := (t_to_Z x <? t_to_Z y)%Z
+       || (((t_to_Z x =? t_to_Z y)%Z)
+             && ((fst x <? fst y)
+                 || ((fst x =? fst y) && (snd x <? snd y)))).
+  Definition leb (x y : t) : bool
+    := ltb x y || ((fst x =? fst y) && (snd x =? snd y)).
+  Theorem leb_total : forall a1 a2, leb a1 a2 = true \/ leb a2 a1 = true.
+  Proof.
+    cbv [leb ltb]; intros a1 a2.
+    repeat first [ rewrite !Bool.andb_true_iff
+                 | rewrite !Bool.orb_true_iff
+                 | rewrite !Z.eqb_eq
+                 | rewrite !Z.ltb_lt
+                 | rewrite !Z.ltb_lt ].
+    destruct (Z.lt_total (t_to_Z a1) (t_to_Z a2)) as [?|[?|?]];
+      try solve [ auto ]; [].
+    destruct (Z.lt_total (fst a1) (fst a2)) as [?|[?|?]];
+      try solve [ auto 6 ]; [].
+    destruct (Z.lt_total (snd a1) (snd a2)) as [?|[?|?]];
+      solve [ auto 7 ].
+  Qed.
+End ZProdOrder.
+
+Module ZProdSort := Sort ZProdOrder.
+Notation Zsort_by_prod := ZProdSort.sort.
+
+Module ZFstOrder <: TotalLeBool.
+  Local Open Scope Z_scope.
+  Definition t := (Z * Z)%type.
+  Definition ltb (x y : t) : bool
+    := (fst x <? fst y)
+       || ((fst x =? fst y)
+             && (snd x <? snd y)).
+  Definition leb (x y : t) : bool
+    := ltb x y || ((fst x =? fst y) && (snd x =? snd y)).
+  Theorem leb_total : forall a1 a2, leb a1 a2 = true \/ leb a2 a1 = true.
+  Proof.
+    cbv [leb ltb]; intros a1 a2.
+    repeat first [ rewrite !Bool.andb_true_iff
+                 | rewrite !Bool.orb_true_iff
+                 | rewrite !Z.eqb_eq
+                 | rewrite !Z.ltb_lt ].
+    destruct (Z.lt_total (fst a1) (fst a2)) as [?|[?|?]];
+      try solve [ auto 6 ]; [].
+    destruct (Z.lt_total (snd a1) (snd a2)) as [?|[?|?]];
+      solve [ auto 7 ].
+  Qed.
+End ZFstOrder.
+
+Module ZFstSort := Sort ZFstOrder.
+Notation Zsort_by_fst := ZFstSort.sort.
+
 Existing Class reflect.
 Notation reflect_rel R1 R2 := (forall x y, reflect (R1 x y) (R2 x y)).
 
@@ -133,6 +190,9 @@ Definition reflect_rel_of_beq_iff {T} {beq : T -> T -> bool} {R : T -> T -> Prop
 Instance reflect_eq_nat : reflect_rel (@eq nat) Nat.eqb
   := reflect_rel_of_beq_iff Nat.eqb_eq.
 
+Instance reflect_eq_Z : reflect_rel (@eq Z) Z.eqb
+  := reflect_rel_of_beq_iff Z.eqb_eq.
+
 Definition remove_smaller_args_of_size_by_reflect
            {T} {T_beq : T -> T -> bool}
            {T_reflect : reflect_rel (@eq T) T_beq}
@@ -142,6 +202,18 @@ Definition remove_smaller_args_of_size_by_reflect
   := let args := uniquify T_beq (args_of_size sz) in
      let smaller_args := flat_map args_of_size (smaller_sizes sz) in
      filter (fun v => negb (existsb (T_beq v) smaller_args)) args.
+
+Class has_sub T := sub : T -> T -> T.
+Instance: has_sub nat := Nat.sub.
+Instance: has_sub Z := Z.sub.
+
+Class has_succ T := succ : T -> T.
+Instance: has_succ nat := S.
+Instance: has_succ Z := Z.succ.
+
+Class has_zero T := zero : T.
+Instance: has_zero nat := O.
+Instance: has_zero Z := Z0.
 
 Ltac default_describe_goal x :=
   idtac "Params: n=" x.
@@ -159,38 +231,30 @@ Ltac runtests args_of_size describe_goal mkgoal redgoal time_solve_goal sz :=
       end in
   iter args.
 
-Ltac do_n tac n start :=
-  lazymatch n with
-  | O => start
-  | S ?n
-    => let n := do_n tac n start in
-       let __ := match goal with _ => tac n end in
-       constr:(S n)
-  | ?v => match goal with
-          | _ => fail 1 "Invalid argument to do_n (expected a literal nat):" v
-          end
-  end.
+Ltac step_goal_from_to step_goal cur_n target_n :=
+  tryif constr_eq cur_n target_n
+  then idtac
+  else let next_n := (eval cbv in (succ cur_n)) in
+       step_goal next_n;
+       step_goal_from_to step_goal next_n target_n.
 
-Ltac runtests_step_arg args_of_size describe_goal mkgoal_step time_solve_goal sz args :=
-  try (assert True;
-       [ once
-           (let n := lazymatch (eval cbv in (option_map args_of_size (size_pred sz))) with
-                     | None => O
-                     | Some ?n => n
-                     end in
-            let start := do_n mkgoal_step n O in
-            let n' := (eval cbv in (args_of_size sz - n)) in
-            do_n
-              ltac:(fun n
-                    => describe_goal n;
-                       try (solve [ once (time_solve_goal n args) ]; []);
-                       mkgoal_step n)
-                     n'
-                     start)
-       | fail ]).
+Ltac runtests_step_arg args_of_size describe_goal step_goal redgoal time_solve_goal sz extra_args :=
+  let args := (eval vm_compute in (remove_smaller_args_of_size_by_reflect sz args_of_size)) in
+  let T := lazymatch type of args with list ?T => T end in
+  let rec iter cur ls :=
+      lazymatch ls with
+      | [] => idtac
+      | ?x :: ?xs
+        => step_goal_from_to step_goal cur x;
+           describe_goal x;
+           try (solve [ redgoal x; once (time_solve_goal x extra_args) ]; []);
+           iter x xs
+      end in
+  let zero := (eval cbv in (@zero T _)) in
+  iter zero args.
 
-Ltac runtests_step args_of_size describe_goal mkgoal_step time_solve_goal sz :=
-  runtests_step_arg args_of_size describe_goal mkgoal_step ltac:(fun n args => time_solve_goal n) sz ().
+Ltac runtests_step args_of_size describe_goal step_goal redgoal time_solve_goal sz :=
+  runtests_step_arg args_of_size describe_goal step_goal redgoal ltac:(fun n args => time_solve_goal n) sz ().
 (*
 Module LiftLetsMap.
   Import Examples.LiftLetsMap.
