performance-experiments-8-9/name_resolution.v
@@ -1,18 +1,19 @@
 Require Import PerformanceExperiments.Harness.
 
-Definition args_of_size (s : size) : nat
+Definition args_of_size (s : size) : list nat
   := match s with
-     | SuperFast => 1500
-     | Fast => 4000
-     | Medium => 4000 + 4000
-     | Slow => 0
-     | VerySlow => 0
+     | SuperFast => seq 0 1500
+     | Fast => seq 0 4000
+     | Medium => seq 0 (4000 + 4000)
+     | Slow => []
+     | VerySlow => []
      end.
 
-Ltac mkgoal_step _ := pose proof I.
+Ltac step_goal _ := pose proof I.
+Ltac redgoal _ := idtac.
 Ltac time_solve_goal0 n tac :=
   time "uconstr-I-1000" (do 1000 let v := tac () in idtac).
-Ltac run0 sz tac := Harness.runtests_step_arg args_of_size default_describe_goal mkgoal_step time_solve_goal0 sz tac.
+Ltac run0 sz tac := Harness.runtests_step_arg args_of_size default_describe_goal step_goal redgoal time_solve_goal0 sz tac.
 (*
 Goal True.
   let tac := ltac:(fun _ => uconstr:(I)) in
