performance-experiments/do_n_open_constr_True.v
@@ -1,0 +1,21 @@
+Require Import PerformanceExperiments.Harness.
+
+Definition args_of_size (s : size) : list nat
+  := match s with
+     | SuperFast => seq 0 300
+     | Fast => (List.map (fun x => x * 2) (seq 0 200))
+                 ++ (List.map (fun x => 400 + 10 * x) (seq 0 30))
+                 ++ (List.map (fun x => 700 + 100 * x) (seq 0 24))
+     | Medium => []
+     | Slow => []
+     | VerySlow => []
+     end.
+
+Ltac step_goal _ := pose proof I.
+Ltac redgoal _ := idtac.
+Ltac time_solve_goal0 n :=
+  time "open-constr-True-1000" (do 1000 let v := open_constr:(_ : True) in idtac).
+Ltac run0 sz := Harness.runtests_step args_of_size default_describe_goal step_goal redgoal time_solve_goal0 sz.
+(*
+Goal True. run0 Fast.
+*)
